Introduce coinductive paths

BinaryRelations.v
@@ -12,6 +12,9 @@ Notation "R ^*" := (clos_refl_trans _ R) (at level 35).
 Definition is_serial {A} (R: relation A) := forall a, exists b, R a b.
 Definition serial A := {R: relation A | is_serial R}.
 
+Definition is_serialT {A} (R: relation A) := forall a, {b | R a b}.
+Definition serialT A := {R: relation A & is_serialT R}.
+
 Definition reachable {A} (R: relation A) (l: list A) (b: A) := exists a, In a l /\ R^* a b.
 
 Inductive steps : nat -> forall {A}, relation A -> relation A :=
