AttarchTrans.v
@@ -7,12 +7,15 @@ Inductive component : Set :=
   | sel4 
   | platam 
   | vmm 
-  | useram.
+  | useram
+  | malicious_linux_component.
 
 Inductive loc : Set :=
   | boot_ev 
   | vm_ev
   | useram_key.
+
+Definition stransition a := transition (sprop component loc) a.
 
 (* Add linux state under vm? *)
 (* Note, all sudoers have access to useram/platam channel *)
@@ -23,12 +26,12 @@ Inductive useram_state : Set :=
   | useram_making_request
   | useram_sending_response.
 
-Inductive useram_trans : transition (sprop component loc) useram_state :=
+Inductive useram_trans : stransition useram_state :=
   | useram_get_key : forall (acc: access component) (k: nat),
       acc useram read ->
       useram_trans
-          (acc @ useram_key ** useram_key ↦ k, useram_waiting_key)
-          (acc @ useram_key ** useram_key ↦ k, useram_waiting_request)
+        (acc @ useram_key ** useram_key ↦ k, useram_waiting_key)
+        (acc @ useram_key ** useram_key ↦ k, useram_waiting_request)
   (* | useram_get_request : useram_trans 
       (s, useram_waiting_key)
       (s,useram_) *)
@@ -42,24 +45,40 @@ Inductive platam_state : Set :=
 
 Definition good_vm_ev : nat. Admitted.
 Definition bad_vm_ev  : nat. Admitted.
-Inductive platam_trans : transition (sprop component loc) platam_state :=
+Definition useram_key_val  : nat. Admitted.
+Inductive useram_key_acc : access component :=
+  | useram_useram_key_read  : useram_key_acc useram read
+  | platam_useram_key_read  : useram_key_acc platam read
+  | platam_useram_key_write : useram_key_acc platam write.
+Inductive platam_trans : stransition platam_state :=
   | platam_measure_good_vm : platam_trans
       (empty, platam_init)
       (private platam @ vm_ev ** vm_ev ↦ good_vm_ev, platam_appraise)
   | platam_measure_bad_vm : platam_trans
       (empty, platam_init)
       (private platam @ vm_ev ** vm_ev ↦ bad_vm_ev, platam_appraise)
-  | platam_appraise_good_vm : forall (acc: access component),
+  | platam_release_key : forall (acc: access component),
       acc platam read ->
       platam_trans
-          (acc @ vm_ev ** vm_ev ↦ good_vm_ev, platam_appraise)
-          (acc @ vm_ev ** vm_ev ↦ good_vm_ev, platam_run).
+        (acc @ vm_ev ** vm_ev ↦ good_vm_ev,
+          platam_appraise)
+        (acc @ vm_ev ** vm_ev ↦ good_vm_ev **
+        useram_key_acc @ useram_key ** useram_key ↦ useram_key_val,
+          platam_run).
 
 Inductive vm_state : Set :=
   | vm_init
   | vm_run : useram_state -> vm_state.
 
-Definition vm_trans : transition (sprop component loc) vm_state. Admitted.
+Inductive vm_trans : stransition vm_state :=
+  | vm_boot : vm_trans
+      (empty, vm_init)
+      (empty, vm_run useram_waiting_key)
+  | vm_linux_step : forall g g' s s',
+      useram_trans (g,s) (g',s') ->
+      vm_trans
+        (g, vm_run s)
+        (g, vm_run s').
 
 Inductive attarch_state : Set :=
   | boot_from_good_plat (* initial state *)
@@ -68,16 +87,16 @@ Inductive attarch_state : Set :=
 
 Definition good_boot_ev : nat. Admitted.
 Definition bad_boot_ev  : nat. Admitted.
-Inductive attarch_trans : transition (sprop component loc) attarch_state :=
+Inductive attarch_trans : stransition attarch_state :=
   | good_boot : attarch_trans 
       (empty, boot_from_good_plat)
-      ((acc_at boot_ev readonly) ** boot_ev ↦ good_boot_ev, sel4_run (platam_init, vm_init))
+      (readonly @ boot_ev ** boot_ev ↦ good_boot_ev, sel4_run (platam_init, vm_init))
   | bad_boot : attarch_trans 
       (empty, boot_from_bad_plat)
-      (acc_at boot_ev readonly ** boot_ev ↦ bad_boot_ev, sel4_run (platam_init, vm_init))
+      (readonly @ boot_ev ** boot_ev ↦ bad_boot_ev, sel4_run (platam_init, vm_init))
   | component_step : forall g g' s s',
       (platam_trans ⊔ vm_trans) (g,s) (g',s') ->
       attarch_trans 
-          (g, sel4_run s)
-          (g', sel4_run s').
-Definition attarch_strans := stransition attarch_trans.
+        (g, sel4_run s)
+        (g', sel4_run s').
+Definition attarch_strans := sprop_closure attarch_trans.
