Ctl/Paths.v
@@ -1,0 +1,116 @@
+Require Import GeneralTactics.
+
+Require Import Coq.Relations.Relation_Definitions.
+
+CoInductive path {state} (R: relation state) (s: state) := 
+  | step : forall s', R s s' -> path R s' -> path R s.
+Arguments step {state R}%type_scope.
+
+(* Definition path_coind {state: Set} {R: relation state}
+  (P: forall s, path R s -> Prop)
+  (coind_step: forall s s' (r : R s s') p, P s' p -> P s (step s s' r p))
+  : forall {s} (p: path R s), (P s p).
+refine (cofix F {s} p := _).
+
+Definition path_coind {state: Set} {R: relation state}
+  (P: forall s, path R s -> Prop)
+  (coind_step: forall s s' (r : R s s') p, P s' p -> P s (step s s' r p)) :=
+  cofix F {s} (p: path R s) : (P s p) :=
+    (* match p as pname return (P s pname) with  *)
+    match p with 
+    | step _ s' r p' => coind_step s s' r p' (F p')
+    end. *)
+
+CoInductive forall_in_path {state R s} (P: state -> Prop) : path R s -> Prop :=
+  | forall_in_step : forall s' r (p: path R s'),
+      P s ->
+      (* Coq infers the wrong value for `s` *)
+      (* forall_path P p -> *)
+      @forall_in_path state R s' P p ->
+      forall_in_path P (step s s' r p).
+
+Inductive in_path {state: Type} {R: relation state} {s} : state -> path R s -> Prop :=
+  | in_head : forall s' r p,
+      in_path s (step s s' r p)
+  | in_tail : forall s' x r p,
+      @in_path state R s' x p ->
+      in_path x (step s s' r p).
+
+Definition forall_in_path' {state: Type} {R: relation state} {s: state}
+  (P: state -> Prop) (p: path R s) :=
+  forall s', in_path s' p -> P s'.
+
+CoInductive exists_in_path {state R s} (P: state -> Prop) : path R s -> Prop :=
+  | exists_in_step : forall s' r (p: path R s'),
+      P s \/ @exists_in_path state R s' P p ->
+      exists_in_path P (step s s' r p).
+
+CoInductive exists_path {state R} (P: state -> Prop) (s: state) : Prop :=
+  | exists_step :
+      P s ->
+      (exists s', R s s' /\ exists_path P s') ->
+      exists_path P s.
+
+(* Require Import Coq.Vectors.VectorDef. *)
+Inductive finite_path {state} (R: relation state) : state -> nat -> Prop := 
+  | finite_trivial : forall s, finite_path R s 0
+  | finite_step : forall s s' n,
+      R s s' ->
+      finite_path R s' n ->
+      finite_path R s (S n).
+Arguments finite_trivial {state R}%type_scope.
+Arguments finite_step    {state R}%type_scope.
+
+Inductive in_finite_path {state} {R: relation state} {s}
+  : state -> forall n: nat, finite_path R s n -> Prop :=
+  | in_finite_head : forall s' n r p,
+      in_finite_path s (S n) (finite_step s s' n r p)
+  | in_finite_tail : forall s' x n r p,
+      @in_finite_path state R s' x n p ->
+      in_finite_path x (S n) (finite_step s s' n r p).
+
+Fixpoint path_to_finite {state} {R: relation state} {s} 
+  (p: path R s) (n: nat) : finite_path R s n :=
+  match n with
+  | 0 => finite_trivial s
+  | S n' =>
+      match p with
+      | step _ s' r p => finite_step s s' n' r (path_to_finite p n')
+      end
+  end.
+
+Lemma in_path_refl_finite {state} {R: relation state} {s} :
+  forall (p: path R s) s',
+  in_path s' p ->
+  exists n, in_finite_path s' n (path_to_finite p n).
+Proof.
+  intros p s' Hin.
+  induction Hin.
+  - exists 1.
+    constructor.
+  - destructExists IHHin n.
+    exists (S n).
+    constructor; assumption.
+Qed.
+
+Theorem forall_in_path_refl_finite {state} {R: relation state} {s}:
+  forall (P: state -> Prop) (p: path R s),
+    (forall n s', in_finite_path s' n (path_to_finite p n) -> P s') ->
+    (forall s', in_path s' p -> P s').
+Proof.
+  intros P p H s' Hin.
+  induction Hin.
+  - apply (H 1).
+    constructor.
+  - apply IHHin.
+    intros n x' H'.
+    apply (H (S n)).
+    constructor; assumption.
+Qed.
+
+Theorem exists_in_path_refl_finite {state} {R: relation state} {s}:
+  forall P (p: path R s),
+    (exists n s', in_finite_path s' n (path_to_finite p n) /\ P s') ->
+    (exists s', in_path s' p /\ P s').
+Proof.
+Admitted.
