Ctl/Properties.v
@@ -1,11 +1,54 @@
-Require Import Coq.Lists.List.
-Import ListNotations.
-Open Scope list_scope.
-Require Import Coq.Relations.Relation_Definitions.
-
+Require Import Ctl.Paths.
 Require Import Ctl.Definition.
 Require Import Ctl.Tactics.
-Require Import Tactics.
+Require Import BinaryRelations.
+Require Import GeneralTactics.
+
+Require Import Coq.Relations.Relation_Definitions.
+Require Import Coq.Relations.Relation_Operators.
+Require Import Coq.Program.Equality.
+
+(* Require Import Coq.Logic.Eqdep_dec. *)
+
+Theorem AG_refl_finite {state}: forall (R: relation state) s P, 
+  (forall s', R^* s s' -> R;s' ⊨ P) ->
+  R;s ⊨ AG P.
+Proof.
+  intros R s P H.
+  intros p s' Hin.
+  apply H.
+  apply in_path_refl_finite in Hin.
+  destruct Hin as [n Hin].
+  (* destruct p as [s'' r p]. *)
+  dependent induction Hin.
+  - apply rt_refl.
+  - 
+    (* simpl in x. *)
+    (* Set Keep Proof Equalities. *)
+    (* injection x. *)
+    eapply rt_trans.
+    + eapply rt_step. eassumption.
+    + 
+      eapply IHHin.
+      * intros s'' HR.
+        apply H.
+        eapply rt_trans.
+        -- eapply rt_step. eassumption.
+        -- assumption.
+      * destruct p as [s'' r' p'].
+        simpl in x.
+        (* assert (finite_path_UIP: forall (x y: finite_path R s (S n)) (p1 p2: x = y), p1 = p2). *)
+        (* assert (finite_path_UIP_refl: forall (x: finite_path R s (S n)) (p: x = x), p = eq_refl x). *)
+        (* { admit. } *)
+        (* apply finite_path_UIP in x. *)
+        admit.
+(* Qed. *)
+Admitted.
+
+  | AG P => forall (p: path R s), forall s', in_path s' p -> R;s' ⊨ P
+  | EG P => exists (p: path R s), forall s', in_path s' p -> R;s' ⊨ P
+  | AF P => forall (p: path R s), exists s', in_path s' p /\ R;s' ⊨ P
+  | EF P => exists (p: path R s), exists s', in_path s' p /\ R;s' ⊨ P
 
 
 Theorem tModusPonens {state}: forall (M: relation state) s P Q,
@@ -17,7 +60,8 @@ Theorem tModusPonens_flipped {state}: forall (M: relation state) s P Q,
 Proof. auto. Qed.
 
 (* Good test for tactics *)
-Theorem TImpl_trans {state}: forall M (s: state) P Q R, M;s ⊨ (P --> Q) --> (Q --> R) --> P --> R.
+Theorem TImpl_trans {state}: forall M (s: state) P Q R,
+  M;s ⊨ (P --> Q) --> (Q --> R) --> P --> R.
 Proof.
   (* backwards reasoning *)
   intros M s P Q R Hpq Hqr Hp.
@@ -43,35 +87,54 @@ Proof.
   split; intros H; auto.
 Qed.
 
-Theorem paths_nonempty {state}: forall (M: relation state) s, exists p, path M (s :: p).
+Theorem path_from_serial {state}: forall (M: serialT state) s, path (projT1 M) s.
 Proof.
-  intros.
-  eexists.
+  intros M.
+  destruct M as [M Hserial]; simpl.
+  cofix coIH.
+  intros s.
+  specialize (Hserial s).
+  destruct Hserial as [s' Hserial].
   econstructor.
+  - eassumption.
+  - auto.
 Qed.
 
-Definition arbitrary_path {state} (M: relation state) s : {π | path M (s :: π)}.
-  repeat econstructor.
-Defined.
+Theorem path_from_serial' {state}:
+  forall (M: relation state), is_serialT M -> forall s, path M s.
+Proof. 
+  intros M Hserial.
+  cofix coIH.
+  intros s.
+  specialize (Hserial s).
+  destruct Hserial as [s' Hserial].
+  econstructor.
+  - eassumption.
+  - auto.
+Qed.
 
 (* De Morgan's Laws *)
 Theorem AF_EG {state}: forall M (s: state) P, M;s ⊨ ¬AF P <--> EG (¬P).
 Proof.
   intros M s P.
-  split.
-  - intros H.
-    exists nil.
-    split; [constructor|].
-    intros s' Hin Hp.
-    inv Hin.
-    tconsume H.
-    eauto.
-  - intros H H2.
-    destruct H as [p [Hpath H]].
-    tspecialize2 H2 p Hpath.
-    destruct H2 as [s' [Hin H2]].
-    specialize (H s').
-    consume H; assumption.
+  split; intro H.
+  - (* Need to construct a path based on contradiction at each step *)
+    simpl. 
+    refine (ex_intro _ (
+      (cofix F s' : path M s' := _) s
+    ) _).
+    intros s' Hin H2.
+    tapply H.
+    intros p.
+    exists s'.
+    split.
+    + 
+    + assumption.
+  - intros H2.
+    destruct H as [p H].
+    tspecialize H2 p.
+    destruct H2 as [s' [HIn H2]].
+    tapply (H s'); assumption.
 Qed.
 
 Theorem AF_EG' {state}: forall M (s: state) P, M;s ⊨ AF (¬P) <--> ¬EG P.
@@ -79,7 +142,7 @@ Admitted.
 
 Theorem EF_AG {state}: forall M (s: state) P, M;s ⊨ ¬EF P <--> AG (¬ P).
 Proof.
-  intros M s P.
+  (* intros M s P.
   split.
   - intros H p Hpath s' Hin H2.
     tconsume H.
@@ -88,7 +151,8 @@ Proof.
     destruct H2 as [p [Hpath [s' [Hin H2]]]].
     tspecialize3 H p Hpath s'.
     tconsume H; assumption.
-Qed.
+Qed. *)
+Admitted.
 
 Theorem AX_EX {state}: forall M (s: state) P, M;s ⊨ ¬AX P <--> EX (¬ P).
 Admitted.
